state/Examples.Intro.fst
@@ -1,28 +1,25 @@
 module Examples.Intro
 
-open FStar.FiniteSet.Base
 open FStar.Ghost
 open FStar.Monotonic.Heap
 open FStar.Preorder
 open FStar.Tactics
 open FStar.Tactics.Typeclasses
 open FStar.Universe
-open STLC
-open Backtranslation.STLCToTargetLang
 open SharedRefs
-open Witnessable
 open HigherOrderContracts
 open TargetLang
 open Compiler
+open Witnessable
 
-type callback =
-  unit -> SST unit (fun _ -> True) (fun h0 _ h1 -> modifies_only_shared_and_encapsulated h0 h1 /\ gets_shared Set.empty h0 h1)
+type callback pspec =
+  mk_targetlang_arrow pspec (raise_t unit) unit (** TODO: why is this raise_t necessary here? **)
 
-type lib_type =
-  r:ref (ref int) -> SST callback (fun _ -> witnessed (contains_pred r) /\ witnessed (is_shared r)) (fun h0 _ h1 -> modifies_only_shared_and_encapsulated h0 h1 /\ gets_shared Set.empty h0 h1)
+type lib_type pspec =
+  mk_targetlang_arrow pspec (ref (ref int)) (callback pspec)
 
 #push-options "--z3rlimit 10000"
-let prog (lib : lib_type) : SST int (requires fun h0 -> True) (ensures fun h0 _ h1 -> True) =
+let prog (lib : lib_type concrete_spec) : SST int (requires fun h0 -> True) (ensures fun h0 _ h1 -> True) =
   let secret : ref int = sst_alloc 42 in
   let r : ref (ref int) = sst_alloc_shared #(SRef SNat) (sst_alloc_shared 0) in
   witness (contains_pred r) ;
@@ -30,32 +27,26 @@ let prog (lib : lib_type) : SST int (requires fun h0 -> True) (ensures fun h0 _ 
   let cb = lib r in
   let v : ref int = sst_alloc_shared 1 in
   sst_write r v;
-  cb ();
+  cb (raise_val ());
   assert (!secret == 42);
   0
 #pop-options
 
 (* Calling SecRef* on it *)
 
-instance imp_cb : safe_importable_to callback = {
-  c_styp = witnessable_arrow unit unit _ _ ;
-  ityp = mk_interm_arrow unit unit ;
-  c_ityp = targetlang_arrow _ unit unit ;
-  safe_import = (fun f x -> f x) ;
-  lemma_safe_import_preserves_prref = (fun x -> ())
-}
-
-instance imp_lib : safe_importable_to lib_type = {
-  c_styp = witnessable_arrow (ref (ref int)) callback _ _ ;
-  ityp = mk_interm_arrow (ref (ref int)) imp_cb.ityp ;
-  c_ityp = targetlang_arrow _ (ref (ref int)) imp_cb.ityp ;
-  safe_import = (fun f r -> imp_cb.safe_import (f r)) ;
-  lemma_safe_import_preserves_prref = (fun f -> ())
-}
-
 let sit : src_interface1 = {
-  ct = lib_type ;
-  c_ct = solve ;
+  ct = lib_type;
+  c_ct = (fun pspec ->
+    safe_importable_arrow_safe
+      pspec
+      (ref (ref int))
+      (callback pspec)
+      #solve
+      #(safe_importable_arrow_safe pspec (raise_t unit) unit _ _ () ())
+      _
+      _
+      ()
+      ());
   psi = fun _ _ _ -> True
 }
 
@@ -67,27 +58,16 @@ let compiled_prog =
 (* Trivial library *)
 
 val triv_lib : ctx_tgt1 (comp_int_src_tgt1 sit)
-let triv_lib #fl inv prref hrel read write alloc r =
-  (fun () -> ())
+let triv_lib inv prref hrel read write alloc r =
+  (fun _ -> ())
 
 let whole_triv : whole_tgt1 =
   link_tgt1 compiled_prog triv_lib
 
 (* Adversarial library *)
 #push-options "--z3rlimit 10000"
-// val adv_lib : ctx_tgt1 (comp_int_src_tgt1 sit)
-let adv_lib_t =
-  #fl: erased tflag ->
-  inv  : (heap -> Type0) ->
-  prref: mref_pred ->
-  hrel : FStar.Preorder.preorder heap ->
-  read :  ttl_read fl inv prref hrel ->
-  write : ttl_write fl inv prref hrel ->
-  alloc : ttl_alloc fl inv prref hrel  ->
-  mk_targetlang_arrow (mk_targetlang_pspec inv prref hrel) (ref (ref int)) (mk_targetlang_arrow (mk_targetlang_pspec inv prref hrel) (raise_t unit) unit)
-val adv_lib : adv_lib_t
-
-let adv_lib #fl inv prref hrel read write alloc r =
+val adv_lib : ctx_tgt1 (comp_int_src_tgt1 sit)
+let adv_lib inv prref hrel read write alloc r =
   let g : ref (linkedList (ref int)) = alloc #(SLList (SRef SNat)) LLNil in
   (* iteration on linked list, using fuel to ensure termination *)
   let pspec = mk_targetlang_pspec inv prref hrel in
@@ -110,17 +90,5 @@ let adv_lib #fl inv prref hrel read write alloc r =
     ()
   )
 
-let pf : squash (adv_lib_t == ctx_tgt1 (comp_int_src_tgt1 sit)) =
-  assert (adv_lib_t == ctx_tgt1 (comp_int_src_tgt1 sit)) by begin
-    norm [delta_only [`%comp_int_src_tgt1; `%Mktgt_interface1?.ct; `%sit; `%adv_lib_t; `%ctx_tgt1];
-          delta_only [`%mk_targetlang_arrow; `%Mksrc_interface1?.c_ct; `%imp_lib; `%Mksafe_importable_to?.ityp];
-          delta_only [`%mk_interm_arrow; `%imp_cb];
-          iota ; Prelude.unascribe];
-    dump "";
-    tadmit()
-  end
-
-// #push-options "--ugly"
 let whole_adv : whole_tgt1 =
-  let _ = pf in
-  link_tgt1 compiled_prog (coerce_eq () (adv_lib <: adv_lib_t))
+  link_tgt1 compiled_prog adv_lib
