state/TargetLang.fst
@@ -12,66 +12,18 @@ instance witnessable_shareable_type (t:Type) {| c:tc_shareable_type t |} : witne
   satisfy = (fun x pred -> forall_refs pred #c.__t x);
 }
 
-(**
-let rec super_lemma (t:shareable_typ) pred x h : Lemma
-  (ensures ((forall_refs_heap pred h #t x) <==> (satisfy_on_heap #(to_Type t) #(witnessable_shareable_type (to_Type t) #(shareable_typ_to_tc t)) x h pred)))
-  [SMTPat (forall_refs_heap pred h #t x); SMTPat (satisfy_on_heap #(to_Type t) #(witnessable_shareable_type (to_Type t) #(shareable_typ_to_tc t)) x h pred)]=
-  match t with
-  | SUnit -> ()
-  | SNat -> ()
-  | SSum t1 t2 -> begin
-    let x : either (to_Type t1) (to_Type t2) = x in
-    match x with
-    | Inl x' -> super_lemma t1 pred x' h
-    | Inr x' -> super_lemma t2 pred x' h
-  end
-  | SRef t' -> begin
-    let x : ref (to_Type t') = x in
-    ()
-  end
-  | SPair t1 t2 -> begin
-    let x : (to_Type t1) * (to_Type t2) = x in
-    super_lemma t1 pred (fst x) h;
-    super_lemma t2 pred (snd x) h
-  end
-  | SLList t' -> begin
-    let x : linkedList (to_Type t') = x in
-    match x with
-    | LLNil -> ()
-    | LLCons v xsref -> super_lemma t' pred v h
-  end
-
-inline_for_extraction
-let sst_alloc #a (#rel:preorder a) (init:a)
-: SST (mref a rel)
-    (fun h0 ->
-      (forall t . to_Type t == a ==>
-        satisfy_on_heap #a #(witnessable_shareable_type a #(shareable_typ_to_tc t)) init h0 contains_pred))
-    (fun h0 r h1 ->
-      alloc_post #a init h0 r h1 /\
-      is_private r h1 /\
-      gets_shared Set.empty h0 h1)
-=
-  let h0 = get_heap () in
-  let r = alloc #a #rel init in
-  let h1 = get_heap () in
-  lemma_fresh_ref_not_shared r h0;
-  lemma_unmodified_map_implies_same_shared_status Set.empty h0 h1;
-  assert (gets_shared Set.empty h0 h1);
-  assert (is_private r h1);
-  assert (alloc_post #a init h0 r h1);
-  assert (ctrans_ref_pred h0 contains_pred);
-  lemma_sst_write_or_alloc_preserves_contains r init h0 h1;
-  lemma_sst_alloc_preserves_shared r init h0 h1;
-  assert (ctrans_ref_pred h1 contains_pred);
-  assert (ctrans_ref_pred h1 is_shared);
-  r
-**)
-
 type targetlang_pspec =
   (inv:heap -> Type0) * (prref:mref_pred) * (hrel:preorder heap)
 
-class targetlang (spec:targetlang_pspec) (t:Type) =
+unfold
+let mk_targetlang_pspec
+  (inv  : heap -> Type0)
+  (prref: mref_pred)
+  (hrel : preorder heap)
+  : targetlang_pspec =
+  (inv, (prref <: (#a:Type0 -> #rel:preorder a -> mref a rel -> Type0)), hrel)
+
+class targetlang (spec:targetlang_pspec) (t:Type u#a) =
   { wt : witnessable t }
 
 instance targetlang_shareable_type pspec (t:Type) {| c:tc_shareable_type t |} : targetlang pspec t = {
@@ -113,8 +65,8 @@ unfold let post_targetlang_arrow
 
 let mk_targetlang_arrow
   (pspec:targetlang_pspec)
-  (t1:Type) {| c1 : witnessable t1 |}
-  (t2:Type) {| c2 : witnessable t2 |}
+  (t1:Type u#a) {| c1 : witnessable t1 |}
+  (t2:Type u#b) {| c2 : witnessable t2 |}
 = x:t1 -> ST t2
     (pre_targetlang_arrow pspec x)
     (post_targetlang_arrow pspec)
@@ -193,9 +145,11 @@ unfold let post_interm_arrow
   (h0:heap) (r:t2) (h1:heap) =
   inv_c h1 /\ h0 `hrel_c` h1 /\ c2.satisfy r prref_c
 
+#set-options "--print_universes"
 let mk_interm_arrow
-  (t1:Type) {| c1 : witnessable t1 |}
-  (t2:Type) {| c2 : witnessable t2 |}
+  (t1:Type u#a) {| c1 : witnessable t1 |}
+  (t2:Type u#b) {| c2 : witnessable t2 |}
+ : Type u#(max 1 a b)
 = x:t1 -> ST t2
     (pre_interm_arrow x)
     (post_interm_arrow)
